Ethereum/Maps/StorageMap.lean
@@ -39,7 +39,7 @@ def Storage.toEthereumStorage (self : Storage) : Ethereum.Storage :=
   self.foldl (init := ∅) λ acc k v ↦ acc.insert (UInt256.ofNat k.1) v
 
 def toBlobs (pair : UInt256 × UInt256) : Option (String × String) := do
-  let kec := ffi.KEC pair.1.toByteArray
+  let kec := KEC pair.1.toByteArray
   let rlp ← RLP (.𝔹 (BE pair.2.toNat))
   pure (Ethereum.toHex kec, Ethereum.toHex rlp)
 
